Source/Dafny/Printer.cs
@@ -1518,7 +1518,7 @@ namespace Microsoft.Dafny {
       } else if (expr is ExprDotName) {
         var e = (ExprDotName)expr;
         // determine if parens are needed
-        int opBindingStrength = 0x80;
+        int opBindingStrength = 0x90;
         bool parensNeeded = !e.Lhs.IsImplicit && // KRML: I think that this never holds
           ParensNeeded(opBindingStrength, contextBindingStrength, fragileContext);
 
@@ -1534,7 +1534,7 @@ namespace Microsoft.Dafny {
       } else if (expr is ApplySuffix) {
         var e = (ApplySuffix)expr;
         // determine if parens are needed
-        int opBindingStrength = 0x80;
+        int opBindingStrength = 0x90;
         bool parensNeeded = !e.Lhs.IsImplicit &&  // KRML: I think that this never holds
           ParensNeeded(opBindingStrength, contextBindingStrength, fragileContext);
 
@@ -1554,7 +1554,7 @@ namespace Microsoft.Dafny {
       } else if (expr is MemberSelectExpr) {
         MemberSelectExpr e = (MemberSelectExpr)expr;
         // determine if parens are needed
-        int opBindingStrength = 0x80;
+        int opBindingStrength = 0x90;
         bool parensNeeded = !e.Obj.IsImplicit &&
           ParensNeeded(opBindingStrength, contextBindingStrength, fragileContext);
 
@@ -1569,7 +1569,7 @@ namespace Microsoft.Dafny {
       } else if (expr is SeqSelectExpr) {
         SeqSelectExpr e = (SeqSelectExpr)expr;
         // determine if parens are needed
-        int opBindingStrength = 0x80;
+        int opBindingStrength = 0x90;
         bool parensNeeded = ParensNeeded(opBindingStrength, contextBindingStrength, fragileContext);
 
         if (parensNeeded) { wr.Write("("); }
@@ -1593,7 +1593,7 @@ namespace Microsoft.Dafny {
       } else if (expr is MultiSelectExpr) {
         MultiSelectExpr e = (MultiSelectExpr)expr;
         // determine if parens are needed
-        int opBindingStrength = 0x80;
+        int opBindingStrength = 0x90;
         bool parensNeeded = ParensNeeded(opBindingStrength, contextBindingStrength, fragileContext);
 
         if (parensNeeded) { wr.Write("("); }
@@ -1617,7 +1617,7 @@ namespace Microsoft.Dafny {
         else
         {
           // determine if parens are needed
-          int opBindingStrength = 0x80;
+          int opBindingStrength = 0x90;
           bool parensNeeded = ParensNeeded(opBindingStrength, contextBindingStrength, fragileContext);
 
           if (parensNeeded) { wr.Write("("); }
@@ -1633,7 +1633,7 @@ namespace Microsoft.Dafny {
       } else if (expr is DatatypeUpdateExpr) {
         var e = (DatatypeUpdateExpr)expr;
         // determine if parens are needed
-        int opBindingStrength = 0x80;
+        int opBindingStrength = 0x90;
         bool parensNeeded = ParensNeeded(opBindingStrength, contextBindingStrength, fragileContext);
 
         if (parensNeeded) { wr.Write("("); }
@@ -1651,7 +1651,7 @@ namespace Microsoft.Dafny {
       } else if (expr is ApplyExpr) {
         var e = (ApplyExpr)expr;
         // determine if parens are needed
-        int opBindingStrength = 0x80;
+        int opBindingStrength = 0x90;
         bool parensNeeded = ParensNeeded(opBindingStrength, contextBindingStrength, fragileContext);
 
         if (parensNeeded) { wr.Write("("); }
@@ -1666,7 +1666,7 @@ namespace Microsoft.Dafny {
       } else if (expr is FunctionCallExpr) {
         var e = (FunctionCallExpr)expr;
         // determine if parens are needed
-        int opBindingStrength = 0x80;
+        int opBindingStrength = 0x90;
         bool parensNeeded = !(e.Receiver.IsImplicit) &&
           ParensNeeded(opBindingStrength, contextBindingStrength, fragileContext);
 
@@ -1716,7 +1716,7 @@ namespace Microsoft.Dafny {
           int opBindingStrength;
           switch (e.Op) {
             case UnaryOpExpr.Opcode.Not:
-              op = "!";  opBindingStrength = 0x70;  break;
+              op = "!";  opBindingStrength = 0x80;  break;
             default:
               Contract.Assert(false); throw new cce.UnreachableException();  // unexpected unary opcode
           }
@@ -1730,10 +1730,14 @@ namespace Microsoft.Dafny {
 
       } else if (expr is ConversionExpr) {
         var e = (ConversionExpr)expr;
+        int opBindingStrength = 0x70;
+        bool parensNeeded = ParensNeeded(opBindingStrength, contextBindingStrength, fragileContext);
+
+        if (parensNeeded) { wr.Write("("); }
+        PrintExpr(e.E, opBindingStrength, false, false, !parensNeeded && isFollowedBySemicolon, -1, keyword);
+        wr.Write(" as ");
         PrintType(e.ToType);
-        wr.Write("(");
-        PrintExpression(e.E, false);
-        wr.Write(")");
+        if (parensNeeded) { wr.Write(")"); }
 
       } else if (expr is BinaryExpr) {
         BinaryExpr e = (BinaryExpr)expr;
@@ -2019,7 +2023,7 @@ namespace Microsoft.Dafny {
       } else if (expr is NegationExpression) {
         var e = (NegationExpression)expr;
         string op = "-";
-        int opBindingStrength = 0x70;
+        int opBindingStrength = 0x80;
         bool parensNeeded = ParensNeeded(opBindingStrength, contextBindingStrength, fragileContext);
 
         if (parensNeeded) { wr.Write("("); }
